src/3d/Desugar.fst
@@ -330,7 +330,7 @@ let resolve_probe_atomic_action (env:qenv) (ac:probe_atomic_action) : ML probe_a
   | Probe_action_copy f v -> Probe_action_copy (resolve_ident env f) (resolve_expr env v)
   | Probe_action_skip n -> Probe_action_skip (resolve_expr env n)
   | Probe_action_fail -> Probe_action_fail
-  
+
 let rec resolve_probe_action' (env:qenv) (act:probe_action') : ML probe_action' =
   match act with
   | Probe_atomic_action ac -> Probe_atomic_action (resolve_probe_atomic_action env ac)
@@ -381,10 +381,11 @@ let resolve_probe_field env = function
   | ProbeDest e -> ProbeDest (resolve_expr env e)
 
 let resolve_probe_call env pc =
-  let { probe_dest; probe_block } = pc in
+  let { probe_dest; probe_block; probe_ptr_as_u64 } = pc in
   {
     probe_dest = resolve_ident env probe_dest;
     probe_block = resolve_probe_action env probe_block;
+    probe_ptr_as_u64 = map_opt (resolve_ident env) probe_ptr_as_u64;
   }
 
 let rec resolve_field (env:qenv) (ff:field) : ML (field & qenv) =
