src/3d/InterpreterTarget.fsti
@@ -193,6 +193,7 @@ type typ : Type =
       sz:A.pointer_size_t ->
       probe:T.probe_action ->
       dest:A.ident ->
+      as_u64:A.ident ->
       typ
 
 val typ_indexes : Type0
